Foundation/Propositional/Boolean/Hilbert.lean
@@ -1,8 +1,8 @@
 module
 
-public import Foundation.Propositional.Hilbert.Standard
-public import Foundation.Propositional.ClassicalSemantics.Basic
+public import Foundation.Propositional.Boolean.Basic
 public import Foundation.Propositional.ConsistentTableau
+public import Foundation.Propositional.Hilbert.Minimal.Basic
 
 @[expose] public section
 
@@ -10,34 +10,40 @@ namespace LO.Propositional
 
 open LO.Entailment
 open Semantics
-open ClassicalSemantics
-open Formula.ClassicalSemantics
+open Boolean
+open Formula.Boolean
 
-namespace Cl
+variable {α} {φ : Formula α}
 
-theorem soundness (h : Propositional.Cl ⊢ φ) : φ.Tautology := by
-  intro v;
+namespace Hilbert.Cl
+
+theorem tautology_of_provable : Hilbert.Cl ⊢ φ → φ.IsTautology := by
+  rintro ⟨h⟩ v;
   induction h with
-  | axm _ h => rcases h with (rfl | rfl) <;> tauto;
-  | mdp ihφψ ihφ => exact ihφψ ihφ;
+  | axm h => rcases h with (⟨_, _, rfl⟩ | ⟨_, _, rfl⟩) <;> tauto;
+  | mdp _ _ ihφψ ihφ => exact ihφψ ihφ;
   | andElimL => simp [Semantics.Models, val]; tauto;
   | andElimR => simp [Semantics.Models, val];
   | orElim => simp [Semantics.Models, val]; tauto;
   | _ => tauto;
+alias soundness := tautology_of_provable
 
-lemma not_provable_of_exists_valuation : (∃ v : Valuation _, ¬(v ⊧ φ)) → Propositional.Cl ⊬ φ := by
+lemma not_provable_of_exists_valuation : (∃ v : Valuation _, ¬(v ⊧ φ)) → Hilbert.Cl ⊬ φ := by
   contrapose!;
-  simpa using soundness;
+  apply tautology_of_provable;
 
-section Completeness
+
+section completeness
 
 open
   Entailment
   SaturatedConsistentTableau
 
-def canonicalVal (T : SaturatedConsistentTableau Propositional.Cl) : Valuation ℕ := λ a => (.atom a) ∈ T.1.1
+variable [DecidableEq α] [Encodable α] {φ : Formula α}
 
-lemma truthlemma {T : SaturatedConsistentTableau Propositional.Cl} : (canonicalVal T) ⊧ φ ↔ φ ∈ T.1.1 := by
+def canonicalVal (T : SaturatedConsistentTableau (Hilbert.Cl : Hilbert α)) : Valuation α := λ a => (.atom a) ∈ T.1.1
+
+lemma truthlemma {T : SaturatedConsistentTableau (Hilbert.Cl : Hilbert α)} : (canonicalVal T) ⊧ φ ↔ φ ∈ T.1.1 := by
   induction φ with
   | hatom => simp [canonicalVal];
   | hfalsum => simp
@@ -82,10 +88,10 @@ lemma truthlemma {T : SaturatedConsistentTableau Propositional.Cl} : (canonicalV
       . left; apply ihφ.mpr hφ;
       . right; apply ihψ.mpr hψ;
 
-theorem completeness : (φ.Tautology) → (Propositional.Cl ⊢ φ) := by
+theorem provable_of_tautology : (φ.IsTautology) → (Hilbert.Cl ⊢ φ) := by
   contrapose;
   intro h;
-  obtain ⟨T, hT⟩ := lindenbaum (𝓢 := Propositional.Cl) (t₀ := (∅, {φ})) $ by
+  obtain ⟨T, hT⟩ := lindenbaum (𝓢 := Hilbert.Cl) (t₀ := (∅, {φ})) $ by
     intro Γ Δ hΓ hΔ;
     by_contra hC;
     apply h;
@@ -98,33 +104,30 @@ theorem completeness : (φ.Tautology) → (Propositional.Cl ⊢ φ) := by
     . simp only [Finset.coe_eq_singleton] at hΔ;
       subst hΔ;
       exact (by simpa using hC) ⨀ verum!;
-  unfold Formula.Tautology Semantics.Valid;
+  dsimp [Formula.IsTautology, Valid];
   push_neg;
   use (canonicalVal T);
   apply truthlemma.not.mpr;
   apply iff_not_mem₁_mem₂.mpr;
   apply hT.2;
   tauto;
+alias completeness := provable_of_tautology
 
 @[grind =]
-theorem iff_provable_tautology : Propositional.Cl ⊢ φ ↔ φ.Tautology := ⟨
-  soundness,
-  completeness,
-⟩
+theorem iff_provable_tautology : Hilbert.Cl ⊢ φ ↔ φ.IsTautology := ⟨soundness, completeness⟩
 
-lemma exists_valuation_of_not_provable : ¬(Propositional.Cl ⊢ φ) → ∃ v : Valuation _, ¬(v ⊧ φ) := by
+lemma exists_valuation_of_not_provable : Hilbert.Cl ⊬ φ → ∃ v : Valuation _, ¬(v ⊧ φ) := by
   contrapose!;
-  simpa using completeness;
+  apply completeness;
 
-end Completeness
+end completeness
 
-theorem tautologies : Propositional.Cl = { φ | φ.Tautology } := by
-  ext;
-  rw [←Logic.iff_provable];
-  apply iff_provable_tautology;
+end Hilbert.Cl
 
-end Cl
-
+@[grind =]
+lemma Cl.iff_mem_tautology [DecidableEq α] [Encodable α] : φ ∈ Propositional.Cl ↔ φ.IsTautology :=
+  Iff.trans Hilbert.iff_mem_logic_provable $ Hilbert.Cl.iff_provable_tautology
 
 end LO.Propositional
+
 end
