Foundation/Modal/Maximal/Unprovability.lean
@@ -38,7 +38,7 @@ end Ver
 
 namespace K4
 
-lemma provable_trivTranslated_Cl : Modal.K4 ⊢ φ → Propositional.Cl ⊢ φᵀ.toPropFormula := by
+lemma provable_trivTranslated_Cl : Modal.K4 ⊢ φ → φᵀ.toPropFormula ∈ Propositional.Cl := by
   intro h;
   apply Triv.iff_provable_Cl.mp;
   apply WeakerThan.pbl h;
@@ -64,7 +64,8 @@ instance : Modal.K4 ⪱ Modal.GL := by
 
 namespace GL
 
-lemma provable_verTranslated_Cl : Modal.GL ⊢ φ → Propositional.Cl ⊢ φⱽ.toPropFormula := by
+lemma provable_verTranslated_Cl : Modal.GL ⊢ φ → φⱽ.toPropFormula ∈ Propositional.Cl := by
+  rw [←Propositional.Hilbert.iff_mem_logic_provable];
   intro h;
   induction h using Hilbert.Normal.rec! with
     | axm _ a =>
