Foundation/Propositional/Logic/Letterless_Int_Cl.lean
@@ -1,9 +1,8 @@
 module
 
-public import Foundation.Modal.Kripke.Logic.S5Grz
-public import Foundation.Modal.Maximal.Makinson
 public import Foundation.Modal.ModalCompanion.Standard.Int
--- public import Foundation.Propositional.Kripke.Logic.Cl
+public import Foundation.Modal.ModalCompanion.Standard.Cl
+public import Foundation.Modal.Maximal.Makinson
 
 @[expose] public section
 
@@ -13,24 +12,21 @@ namespace LO.Propositional
 lemma Formula.gödelTranslate.Letterless {φ : Formula ℕ} (hφ : φ.Letterless) : φᵍ.Letterless := by
   induction φ <;> . simp_all only [Formula.gödelTranslate]; grind;
 
-namespace Logic
+open LO.Entailment LO.Modal.Entailment
 
-open LO.Entailment LO.Entailment.FiniteContext LO.Modal.Entailment
-
-theorem iff_letterless_Int_Cl {φ : Formula ℕ} (hφ : φ.Letterless) : Propositional.Int ⊢ φ ↔ Propositional.Cl ⊢ φ := by
+theorem iff_letterless_Int_Cl {φ : Formula ℕ} (hφ : φ.Letterless) : φ ∈ Propositional.Int ↔ φ ∈ Propositional.Cl := by
   constructor;
   . apply WeakerThan.wk;
     infer_instance;
   . intro h;
-    have : Modal.S4 ⊢ ◇φᵍ := Modal.iff_provable_Cl_provable_dia_gS4.mp h;
-    have : Modal.Triv ⊢ ◇φᵍ := WeakerThan.pbl this;
-    have : Modal.Triv ⊢ φᵍ := diaT'! this;
-    have : (φᵍᵀ.toPropFormula _).Tautology := Modal.Triv.iff_tautology.mp this;
-    have : Modal.KD ⊢ φᵍ := Modal.Logic.provable_KD_of_classical_tautology (by grind) this;
-    have : Modal.S4 ⊢ φᵍ := WeakerThan.pbl this;
-    exact Modal.ModalCompanion.companion.mpr this;
-
-end Logic
+    apply Propositional.Int.modalCompanion_S4.mpr
+      $ WeakerThan.pbl
+      $ Modal.Logic.provable_KD_of_classical_tautology (by grind)
+      $ Modal.Triv.iff_tautology.mp
+      $ diaT'!
+      $ WeakerThan.pbl
+      $ Cl.iff_mem_S4_dia.mp h;
 
 end LO.Propositional
+
 end
