Foundation/Propositional/Logic/PostComplete.lean
@@ -1,7 +1,7 @@
 module
 
-public import Foundation.Propositional.ClassicalSemantics.Hilbert
-public import Foundation.Propositional.ClassicalSemantics.ZeroSubst
+public import Foundation.Propositional.Boolean.Hilbert
+public import Foundation.Propositional.Boolean.ZeroSubst
 
 @[expose] public section
 
@@ -9,24 +9,26 @@ namespace LO.Propositional
 
 -- abbrev Ext (L : Logic ℕ) := { L' : Logic ℕ // L'.Superintuitionistic }
 
-open Formula (atom)
-open Formula.ClassicalSemantics
-open Cl
-open ClassicalSemantics
+variable {α} [DecidableEq α] [Encodable α]
 
-theorem Cl.post_complete : ¬∃ L : Logic _, Entailment.Consistent L ∧ Nonempty (L.Superintuitionistic) ∧ Propositional.Cl ⪱ L := by
+open Formula (atom)
+open Formula.Boolean
+open Cl
+open Boolean
+
+theorem Cl.post_complete : ¬∃ L : SuperintuitionisticLogic α, L.Consistent ∧ Propositional.Cl.logic ⊂ L.logic := by
   by_contra! hC;
-  obtain ⟨L, L_consis, ⟨L_ne⟩, L_Cl⟩ := hC;
-  apply Logic.no_bot (L := L);
-  obtain ⟨hL, φ, hφ₁, hφ₂⟩ := Entailment.strictlyWeakerThan_iff.mp L_Cl;
-  have ⟨v, hv⟩ := exists_valuation_of_not_provable hφ₁;
-  have h₁ : L ⊢ ∼(φ⟦(vfSubst v).1⟧) := hL $ by
-    apply iff_provable_tautology.mpr;
-    apply neg_tautology_of_letterless_of_tautology;
+  obtain ⟨L, L_consis, L_Cl⟩ := hC;
+  apply L.not_mem_bot;
+  obtain ⟨hL, φ, hφ₁, hφ₂⟩ := Set.ssubset_iff_exists.mp L_Cl;
+  have ⟨v, hv⟩ := Hilbert.Cl.exists_valuation_of_not_provable hφ₂;
+  have h₁ : ∼(φ⟦(vfSubst v).1⟧) ∈ L.logic := hL $ by
+    apply Hilbert.Cl.iff_provable_tautology.mpr;
+    apply Formula.neg_isTautology_of_letterless_of_isTautology;
     . grind;
     . apply vfSubst_tautology.not.mp hv;
-  have h₂ : L ⊢ φ⟦(vfSubst v).1⟧ := L.subst _ hφ₂;
-  exact h₁ ⨀ h₂;
+  have h₂ : (φ⟦(vfSubst v).1⟧) ∈ L.logic := L.subst _ _ hφ₁;
+  exact L.mdp h₁ h₂;
 
 end LO.Propositional
 end
